@prefix rdf: <http://www.w3.org/1999/02/22-rdf-syntax-ns#> .
@prefix rdfs: <http://www.w3.org/2000/01/rdf-schema#> .
@prefix uostr: <https://w3id.org/DigiTwin/TestRun#> .
@prefix xsd: <http://www.w3.org/2001/XMLSchema#> .
@prefix iotics:  <http://data.iotics.com/iotics#> .
@prefix uom: <http://www.ontology-of-units-of-measure.org/resource/om-2/> .
@prefix geosp: <http://www.opengis.net/ont/geosparql#> .
@prefix dct: <http://purl.org/dc/terms/> .

# Classes
uostr:TestRun
  a rdfs:Class ;
  rdfs:label "A single run of experiments." ;
  rdfs:comment "An experimental run with a specific experimental configuration." ;
.

uostr:TestType
  a rdfs:Class ;
  rdfs:label "Type of test" ;
  rdfs:comment "Type of test regarding the excitation force used." ;
.

uostr:SingleShakerExcitationTest
  a rdfs:Class ;
  rdfs:subClassOf uostr:TestType ;
  rdfs:label "A test using a single shaker." ;
  rdfs:comment "A test with only one mechanical shaker to excite the structure." ;
.
uostr:MultipleShakerExcitationTest
  a rdfs:Class ;
  rdfs:subClassOf uostr:TestType ;
  rdfs:label "A test using multiple shaker." ;
  rdfs:comment "A test with more than one mechanical shaker to excite the structure." ;
.

uostr:BurstRandom
  a uostr:SingleShakerExcitationTest;
  rdfs:label "A test using a burst random excitation." ;
  rdfs:comment "A single shaker test, whose excitatation force is a burst random excitation." ;
.

uostr:ContinuousRandom
  a uostr:SingleShakerExcitationTest ;
  rdfs:label "A test using a continuous random excitation." ;
  rdfs:comment "A single shaker test, whose excitatation force is a continuously random signal also known as white-noise or pseudo-random excitation." ;
.

uostr:SineSwept
  a uostr:SingleShakerExcitationTest ;
  rdfs:label "A test using a sine swept excitation." ;
  rdfs:comment "A single shaker test with a single frequency excitation, whose excitatation frequency changes as a function of time." ;
.

uostr:AddedMass
  a rdfs:Class ;
  rdfs:label "The added-on-the-structure mass during the run." ;
  rdfs:comment "The value and position of the mass, which was added on the structure during the run, often in order to immitate the existence of damage or nonlinearity." ;
.

uostr:CoordinatesArray
  a rdfs:Class ;
  rdfs:label "Array of coordinates in a 3D euclidean space" ;
  rdfs:comment "Coordinates in a 3D euclidean space" ;
.

uostr:MassArray
  a rdfs:Class ;
  rdfs:label "Array of added masses during a run." ;
  rdfs:comment "Array of masses in kg" ;
.

uostr:ControlFramework
  a rdfs:Class ;
  rdfs:label "Control of shaker output in frequency domain" ;
  rdfs:comment "The control framework used to control the mechanical shaker during the run." ;
.

uostr:ClosedLoopControlFramework
  a uostr:ControlFramework ;
  rdfs:label "Closed loop control of shaker output in frequency domain." ;
  rdfs:comment "A control framework that utilises real-time information to modulate the excitation to a desired output." ;
.

uostr:OpenLoopControlFramework
  a uostr:ControlFramework ;
  rdfs:label "Open loop control of shaker output in frequency domain" ;
  rdfs:comment "A control framework that uses a pre-determined signal to excite the system." ;
.

# Properties of Classes, domain base of link and range tip of arrow. No domain means can be applied to multiple classes
uostr:hasTestType
  a rdf:property;
  rdfs:domain uostr:TestRun;
  rdfs:range uostr:TestType;
  rdfs:label "Specify excitation type";
.

uostr:hasAmplificationLevel
  a rdf:property ;
  rdfs:domain uostr:TestRun ;
  rdfs:range xsd:float ;
  rdfs:label "Power amplification from LMS to Shaker" ;
.

uostr:hasBandwidth
  a rdf:property ;
  rdfs:domain uostr:TestRun ;
  rdfs:range xsd:float ;
  rdfs:label "Frequency Bandwidth" ;
.

uostr:hasAddedMasses
  a rdf:property ;
  rdfs:domain uostr:TestRun ;
  rdfs:range uostr:AddedMass ;
  rdfs:label "Specify if there are added masses" ;
.

uostr:hasMassLocations
  a rdf:property;
  rdfs:domain uostr:AddedMass ;
  rdfs:range uostr:CoordinatesArray;
  rdfs:label "Location of masses";
.

uostr:hasMassValues
  a rdf:property ;
  rdfs:domain uostr:AddedMass ;
  rdfs:range uostr:MassArray ;
  rdfs:label "The mass added at a specific points for an experiment" ;
.

uostr:hasSpectralLines
  a rdf:property;
  rdfs:domain uostr:TestRun ;
  rdfs:range xsd:integer;
  rdfs:label "Number of frequencies in FRF";
.

uostr:hasNumberOfAverages
  a rdf:property;
  rdfs:domain uostr:TestRun ;
  rdfs:range xsd:integer ;
  rdfs:label "Number of FRF windows for averaging";
.

uostr:hasControlFramework
  a rdf:property;
  rdfs:domain uostr:TestRun ;
  rdfs:range uostr:ControlFramework;
  rdfs:label "Specify Control";
.

uostr:hasRepetitionIndex
  a rdf:property;
  rdfs:domain uostr:TestRun ;
  rdfs:range xsd:integer ;
  rdfs:label "Set index for repetitions";
.

uostr:hasAdditionalNotes
  a rdf:property;
  rdfs:domain uostr:TestRun ;
  rdfs:range xsd:string ;
  rdfs:label "Added Notes";
.
